avltree/BinTree.lean
@@ -6,29 +6,30 @@ inductive BinTree : Type
 
 @[simp]
 def size : BinTree → Nat
-  | .empty       => 0
-  | .node _ l r  => 1 + size l + size r
+  | .empty              => 0
+  | .node _ left right  => 1 + size left + size right
 
 @[simp]
 def height : BinTree → Nat
-  | .empty       => 0
-  | .node _ l r  => 1 + max (height l) (height r)
+  | .empty              => 0
+  | .node _ left right  => 1 + max (height left) (height right)
 
 @[simp]
-def insert_left (x : Nat) (t : BinTree) : BinTree :=
-  match t with
-  | .empty       => .node x .empty .empty
-  | .node v l r  => .node x (.node v l r) .empty
+def insert_left (value : Nat) (tree : BinTree) : BinTree :=
+  match tree with
+  | .empty                     => .node value .empty .empty
+  | .node nodeValue left right => .node value (.node nodeValue left right) .empty
 
 @[simp]
-def insert_right (x : Nat) (t : BinTree) : BinTree :=
-  match t with
-  | .empty       => .node x .empty .empty
-  | .node v l r  => .node x .empty (.node v l r)
+def insert_right (value : Nat) (tree : BinTree) : BinTree :=
+  match tree with
+  | .empty                     => .node value .empty .empty
+  | .node nodeValue left right => .node value .empty (.node nodeValue left right)
 
 @[simp]
-def collect : BinTree → List Nat
-  | .empty       => []
-  | .node v l r  => collect l ++ [v] ++ collect r
+def collect_values : BinTree → List Nat
+  | .empty              => []
+  | .node value left right  =>
+      collect_values left ++ [value] ++ collect_values right
 
 end BinTree
